README.md
@@ -3,4 +3,47 @@ Precise Reasoning with Structured Time, Structured Heaps, and Collective Operati
 
 Program analysis by optimizing for clarity.
 
-(TODO: document Coq proofs and implementation)
+## Coq Proof
+
+### Definition and modelization
+
+#### IMP
+
+ - IMP language [(Figure 3)](coq/IMP.v#L74)
+ - IMP Relational big-step semantic (Figure 4)
+   * [Expression Evaluation](coq/IMP.v#L325)
+   * [Loop Evaluation](coq/IMP.v#L368)
+   * [Statement Evaluation](coq/IMP.v#L377)
+ - IMP functonal semantics (Figure 5)
+   * [Expression Evaluation](coq/IMP.v#L592)
+   * [Loop Evaluation](coq/IMP.v#L654)
+   * [Statement Evaluation](coq/IMP.v#L668)
+
+#### FUN
+
+ - FUN language [(Figure 6)](coq/FUN.v#L14)
+ - FUN value representation for Option Monad [(Figure 7)](coq/FUN.v#L39)
+ - FUN small [step semantics](coq/FUN.v#L258)
+
+#### IMP to FUN transformation
+
+   * [Expression Transformation](coq/FUN.v#L137)
+   * [Statement Transformation](coq/FUN.v#L169)
+   * [Equivalence](coq/FUN.v#L435)
+
+### Theorems
+
+ - IMP is deterministic
+    * [Expression Deterministic](coq/IMP.v#L410)
+    * [Proposition 3.3](coq/IMP.v#L466)
+
+ - Adequacy between big-step semantics and functional semantics.
+    * [Expression Adequacy](coq/IMP.v#L714)
+    * [Statement Adequacy (1st half)](coq/IMP.v#L1009)
+    * [Statement Adequacy (2nd half)](coq/IMP.v#L1182)
+    * [Proposition 3.9](coq/IMP.v#1255)
+
+  - Soundness of the IMP to FUN transformation
+    * [Expression Soundness](coq/FUN.v#L1316)
+    * [Statement Soundness](coq/FUN.v#L2066)
+    * [Theorem 3.14](coq/FUN.v#L2299)
